Mlir/Rewriter/LinkedList/GetSet.lean
@@ -37,7 +37,7 @@ import Mlir.Rewriter.LinkedList.Basic
  -/
 namespace Mlir
 
-variable {operation operation' : OperationPtr}
+variable {op op' operation operation' : OperationPtr}
 variable {block block' : BlockPtr}
 variable {rg rg' : RegionPtr}
 variable {opOperand opOperand' : OpOperandPtr}
@@ -476,234 +476,683 @@ theorem OpOperandPtrPtr.get!_OpOperandPtr_insertIntoCurrent {opOperandPtr : OpOp
       opOperandPtr.get! ctx := by
   grind
 
-@[simp, grind =>]
-theorem OperationPtr.get!_OperationPtr_setParentWithCheck
-    (heq : operation'.setParentWithCheck ctx parent h' = some newCtx) :
-    operation.get! newCtx =
-    if operation' = operation then
-      { operation.get! ctx with parent := some parent }
+/- OperationPtr.linkBetween -/
+section linkBetween
+attribute [local grind] OperationPtr.linkBetween
+
+@[simp, grind =]
+theorem IRContext.topLevelOp_OperationPtr_linkBetween :
+    (op'.linkBetween ctx prev next selfIn prevIn nextIn).topLevelOp =
+    ctx.topLevelOp := by
+  -- TODO: Why does grind need an explicit unfold here?
+  simp only [OperationPtr.linkBetween]
+  grind
+
+@[simp, grind =]
+theorem BlockPtr.get!_OperationPtr_linkBetween {block : BlockPtr} :
+    block.get! (op'.linkBetween ctx prev next selfIn prevIn nextIn) =
+    block.get! ctx := by
+  simp only [OperationPtr.linkBetween]
+  grind
+
+@[grind =]
+theorem OperationPtr.prev!_OperationPtr_linkBetween {operation : OperationPtr} :
+    (operation.get! (op'.linkBetween ctx prev next selfIn prevIn nextIn)).prev =
+    if operation = next then
+      some op'
+    else if operation = op' then
+      prev
     else
-      operation.get! ctx
+      (operation.get! ctx).prev := by
+  simp only [OperationPtr.linkBetween]
+  grind
+
+@[grind =]
+theorem OperationPtr.next!_OperationPtr_linkBetween {operation : OperationPtr} :
+    (operation.get! (op'.linkBetween ctx prev next selfIn prevIn nextIn)).next =
+    if operation = prev then
+      some op'
+    else if operation = op' then
+      next
+    else
+      (operation.get! ctx).next := by
+  simp only [OperationPtr.linkBetween]
+  grind
+
+@[simp, grind =]
+theorem OperationPtr.parent!_OperationPtr_linkBetween {operation : OperationPtr} :
+    (operation.get! (op'.linkBetween ctx prev next selfIn prevIn nextIn)).parent =
+    (operation.get! ctx).parent := by
+  simp only [OperationPtr.linkBetween]
+  grind
+
+@[simp, grind =]
+theorem OperationPtr.opType!_OperationPtr_linkBetween {operation : OperationPtr} :
+    (operation.get! (op'.linkBetween ctx prev next selfIn prevIn nextIn)).opType =
+    (operation.get! ctx).opType := by
+  simp only [OperationPtr.linkBetween]
+  grind
+
+@[simp, grind =]
+theorem OperationPtr.attrs!_OperationPtr_linkBetween {operation : OperationPtr} :
+    (operation.get! (op'.linkBetween ctx prev next selfIn prevIn nextIn)).attrs =
+    (operation.get! ctx).attrs := by
+  grind
+
+@[simp, grind =]
+theorem OperationPtr.properties!_OperationPtr_linkBetween {operation : OperationPtr} :
+    (operation.get! (op'.linkBetween ctx prev next selfIn prevIn nextIn)).properties =
+    (operation.get! ctx).properties := by
+  simp only [OperationPtr.linkBetween]
+  grind
+
+@[simp, grind =]
+theorem OperationPtr.getNumResults!_OperationPtr_linkBetween {operation : OperationPtr} :
+    operation.getNumResults! (op'.linkBetween ctx prev next selfIn prevIn nextIn) =
+    operation.getNumResults! ctx := by
+  simp only [OperationPtr.linkBetween]
+  grind
+
+@[simp, grind =]
+theorem OpResultPtr.get!_OperationPtr_linkBetween {opResult : OpResultPtr} :
+    opResult.get! (op'.linkBetween ctx prev next selfIn prevIn nextIn) =
+    opResult.get! ctx := by
+  simp only [OperationPtr.linkBetween]
+  grind
+
+@[simp, grind =]
+theorem OperationPtr.getNumOperands!_OperationPtr_linkBetween {operation : OperationPtr} :
+    operation.getNumOperands! (op'.linkBetween ctx prev next selfIn prevIn nextIn) =
+    operation.getNumOperands! ctx := by
+  simp only [OperationPtr.linkBetween]
+  grind
+
+@[simp, grind =]
+theorem OpOperandPtr.get!_OperationPtr_linkBetween {opOperand : OpOperandPtr} :
+    opOperand.get! (op'.linkBetween ctx prev next selfIn prevIn nextIn) =
+    opOperand.get! ctx := by
+  simp only [OperationPtr.linkBetween]
+  grind
+
+@[simp, grind =]
+theorem OperationPtr.getNumSuccessors!_OperationPtr_linkBetween {operation : OperationPtr} :
+    operation.getNumSuccessors! (op'.linkBetween ctx prev next selfIn prevIn nextIn) =
+    operation.getNumSuccessors! ctx := by
+  simp only [OperationPtr.linkBetween]
+  grind
+
+@[simp, grind =]
+theorem BlockOperandPtr.get!_OperationPtr_linkBetween {blockOperand : BlockOperandPtr} :
+    blockOperand.get! (op'.linkBetween ctx prev next selfIn prevIn nextIn) =
+    blockOperand.get! ctx := by
+  simp only [OperationPtr.linkBetween]
+  grind
+
+@[simp, grind =]
+theorem OperationPtr.getNumRegions!_OperationPtr_linkBetween {operation : OperationPtr} :
+    operation.getNumRegions! (op'.linkBetween ctx prev next selfIn prevIn nextIn) =
+    operation.getNumRegions! ctx := by
+  simp only [OperationPtr.linkBetween]
+  grind
+
+@[simp, grind =]
+theorem OperationPtr.getRegion!_OperationPtr_linkBetween {operation : OperationPtr} :
+    operation.getRegion! (op'.linkBetween ctx prev next selfIn prevIn nextIn) =
+    operation.getRegion! ctx := by
+  simp only [OperationPtr.linkBetween]
+  grind
+
+@[simp, grind =]
+theorem BlockOperandPtrPtr.get!_OperationPtr_linkBetween {blockOperandPtr : BlockOperandPtrPtr} :
+    blockOperandPtr.get! (op'.linkBetween ctx prev next selfIn prevIn nextIn) =
+    blockOperandPtr.get! ctx := by
+  simp only [OperationPtr.linkBetween]
+  grind
+
+@[simp, grind =]
+theorem BlockPtr.getNumArguments!_OperationPtr_linkBetween {block : BlockPtr} :
+    block.getNumArguments! (op'.linkBetween ctx prev next selfIn prevIn nextIn) =
+    block.getNumArguments! ctx := by
+  simp only [OperationPtr.linkBetween]
+  grind
+
+@[simp, grind =]
+theorem BlockArgumentPtr.get!_OperationPtr_linkBetween {blockArg : BlockArgumentPtr} :
+    blockArg.get! (op'.linkBetween ctx prev next selfIn prevIn nextIn) =
+    blockArg.get! ctx := by
+  simp only [OperationPtr.linkBetween]
+  grind
+
+@[simp, grind =]
+theorem RegionPtr.get!_OperationPtr_linkBetween {region : RegionPtr} :
+    region.get! (op'.linkBetween ctx prev next selfIn prevIn nextIn) =
+    region.get! ctx := by
+  simp only [OperationPtr.linkBetween]
+  grind
+
+@[simp, grind =]
+theorem ValuePtr.getFirstUse!_OperationPtr_linkBetween {value : ValuePtr} :
+    value.getFirstUse! (op'.linkBetween ctx prev next selfIn prevIn nextIn) =
+    value.getFirstUse! ctx := by
+  simp only [OperationPtr.linkBetween]
+  grind
+
+@[simp, grind =]
+theorem ValuePtr.getType!_OperationPtr_linkBetween {value : ValuePtr} :
+    value.getType! (op'.linkBetween ctx prev next selfIn prevIn nextIn) =
+    value.getType! ctx := by
+  grind
+
+@[simp, grind =]
+theorem OpOperandPtrPtr.get!_OperationPtr_linkBetween {opOperandPtr : OpOperandPtrPtr} :
+    opOperandPtr.get! (op'.linkBetween ctx prev next selfIn prevIn nextIn) =
+    opOperandPtr.get! ctx := by
+  simp only [OperationPtr.linkBetween]
+  grind
+
+end linkBetween
+
+section setParentWithCheck
+
+/- OperationPtr.setParentWithCheck -/
+attribute [local grind] OperationPtr.setParentWithCheck
+
+@[simp]
+theorem IRContext.topLevelOp_OperationPtr_setParentWithCheck :
+    op'.setParentWithCheck ctx newParent selfIn = some newCtx →
+    newCtx.topLevelOp = ctx.topLevelOp := by
+  grind
+
+grind_pattern IRContext.topLevelOp_OperationPtr_setParentWithCheck =>
+  op'.setParentWithCheck ctx newParent selfIn, some newCtx, newCtx.topLevelOp
+
+@[simp]
+theorem BlockPtr.get!_OperationPtr_setParentWithCheck {block : BlockPtr} :
+    op'.setParentWithCheck ctx newParent selfIn = some newCtx →
+    (block.get! newCtx) = (block.get! ctx) := by
+  grind
+
+grind_pattern BlockPtr.get!_OperationPtr_setParentWithCheck =>
+  op'.setParentWithCheck ctx newParent selfIn, some newCtx, block.get! newCtx
+
+@[simp]
+theorem OperationPtr.prev!_OperationPtr_setParentWithCheck {operation : OperationPtr} :
+    op'.setParentWithCheck ctx newParent selfIn = some newCtx →
+    (operation.get! newCtx).prev = (operation.get! ctx).prev := by
+  grind
+
+grind_pattern OperationPtr.prev!_OperationPtr_setParentWithCheck =>
+  op'.setParentWithCheck ctx newParent selfIn, some newCtx, (operation.get! newCtx).prev
+
+@[simp]
+theorem OperationPtr.next!_OperationPtr_setParentWithCheck {operation : OperationPtr} :
+    op'.setParentWithCheck ctx newParent selfIn = some newCtx →
+    (operation.get! newCtx).next = (operation.get! ctx).next := by
+  simp only [OperationPtr.setParentWithCheck]
+  grind
+
+grind_pattern OperationPtr.next!_OperationPtr_setParentWithCheck =>
+  op'.setParentWithCheck ctx newParent selfIn, some newCtx, (operation.get! newCtx).next
+
+theorem OperationPtr.parent!_OperationPtr_setParentWithCheck {operation : OperationPtr} :
+    op'.setParentWithCheck ctx newParent selfIn = some newCtx →
+    (operation.get! newCtx).parent =
+    if operation = op' then
+      some newParent
+    else
+      (operation.get! ctx).parent := by
+  grind
+
+grind_pattern OperationPtr.parent!_OperationPtr_setParentWithCheck =>
+  op'.setParentWithCheck ctx newParent selfIn, some newCtx, (operation.get! newCtx).parent
+
+@[simp]
+theorem OperationPtr.opType!_OperationPtr_setParentWithCheck {operation : OperationPtr} :
+    op'.setParentWithCheck ctx newParent selfIn = some newCtx →
+    (operation.get! newCtx).opType = (operation.get! ctx).opType := by
+  grind
+
+grind_pattern OperationPtr.opType!_OperationPtr_setParentWithCheck =>
+  op'.setParentWithCheck ctx newParent selfIn, some newCtx, (operation.get! newCtx).opType
+
+@[simp]
+theorem OperationPtr.attrs!_OperationPtr_setParentWithCheck {operation : OperationPtr} :
+    op'.setParentWithCheck ctx newParent selfIn = some newCtx →
+    (operation.get! newCtx).attrs = (operation.get! ctx).attrs := by
+  grind
+
+grind_pattern OperationPtr.attrs!_OperationPtr_setParentWithCheck =>
+  op'.setParentWithCheck ctx newParent selfIn, some newCtx, (operation.get! newCtx).attrs
+
+@[simp]
+theorem OperationPtr.properties!_OperationPtr_setParentWithCheck {operation : OperationPtr} :
+    op'.setParentWithCheck ctx newParent selfIn = some newCtx →
+    (operation.get! newCtx).properties = (operation.get! ctx).properties := by
+  grind
+
+grind_pattern OperationPtr.properties!_OperationPtr_setParentWithCheck =>
+  op'.setParentWithCheck ctx newParent selfIn, some newCtx, (operation.get! newCtx).properties
+
+@[simp]
+theorem OperationPtr.getNumResults!_OperationPtr_setParentWithCheck {operation : OperationPtr} :
+    op'.setParentWithCheck ctx newParent selfIn = some newCtx →
+    operation.getNumResults! newCtx = operation.getNumResults! ctx := by
+  grind
+
+grind_pattern OperationPtr.getNumResults!_OperationPtr_setParentWithCheck =>
+  op'.setParentWithCheck ctx newParent selfIn, some newCtx, operation.getNumResults! newCtx
+
+@[simp]
+theorem OpResultPtr.get!_OperationPtr_setParentWithCheck {opResult : OpResultPtr} :
+    op'.setParentWithCheck ctx newParent selfIn = some newCtx →
+    opResult.get! newCtx = opResult.get! ctx := by
+  grind
+
+grind_pattern OpResultPtr.get!_OperationPtr_setParentWithCheck =>
+  op'.setParentWithCheck ctx newParent selfIn, some newCtx, opResult.get! newCtx
+
+@[simp]
+theorem OperationPtr.getNumOperands!_OperationPtr_setParentWithCheck {operation : OperationPtr} :
+    op'.setParentWithCheck ctx newParent selfIn = some newCtx →
+    operation.getNumOperands! newCtx = operation.getNumOperands! ctx := by
+  grind
+
+grind_pattern OperationPtr.getNumOperands!_OperationPtr_setParentWithCheck =>
+  op'.setParentWithCheck ctx newParent selfIn, some newCtx, operation.getNumOperands! newCtx
+
+@[simp]
+theorem OpOperandPtr.get!_OperationPtr_setParentWithCheck {operand : OpOperandPtr} :
+    op'.setParentWithCheck ctx newParent selfIn = some newCtx →
+    operand.get! newCtx = operand.get! ctx := by
+  grind
+
+grind_pattern OpOperandPtr.get!_OperationPtr_setParentWithCheck =>
+  op'.setParentWithCheck ctx newParent selfIn, some newCtx, operand.get! newCtx
+
+@[simp]
+theorem OperationPtr.getNumSuccessors!_OperationPtr_setParentWithCheck {operation : OperationPtr} :
+    op'.setParentWithCheck ctx newParent selfIn = some newCtx →
+    operation.getNumSuccessors! newCtx = operation.getNumSuccessors! ctx := by
+  grind
+
+grind_pattern OperationPtr.getNumSuccessors!_OperationPtr_setParentWithCheck =>
+  op'.setParentWithCheck ctx newParent selfIn, some newCtx, operation.getNumSuccessors! newCtx
+
+@[simp]
+theorem BlockOperandPtr.get!_OperationPtr_setParentWithCheck {operand : BlockOperandPtr} :
+    op'.setParentWithCheck ctx newParent selfIn = some newCtx →
+    operand.get! newCtx = operand.get! ctx := by
+  grind
+
+grind_pattern BlockOperandPtr.get!_OperationPtr_setParentWithCheck =>
+  op'.setParentWithCheck ctx newParent selfIn, some newCtx, operand.get! newCtx
+
+@[simp]
+theorem OperationPtr.getNumRegions!_OperationPtr_setParentWithCheck {operation : OperationPtr} :
+    op'.setParentWithCheck ctx newParent selfIn = some newCtx →
+    operation.getNumRegions! newCtx = operation.getNumRegions! ctx := by
+  grind
+
+grind_pattern OperationPtr.getNumRegions!_OperationPtr_setParentWithCheck =>
+  op'.setParentWithCheck ctx newParent selfIn, some newCtx, operation.getNumRegions! newCtx
+
+@[simp]
+theorem OperationPtr.getRegion!_OperationPtr_setParentWithCheck {operation : OperationPtr} :
+    op'.setParentWithCheck ctx newParent selfIn = some newCtx →
+    operation.getRegion! newCtx = operation.getRegion! ctx := by
+  grind
+
+grind_pattern OperationPtr.getRegion!_OperationPtr_setParentWithCheck =>
+  op'.setParentWithCheck ctx newParent selfIn, some newCtx, operation.getRegion! newCtx
+
+@[simp]
+theorem BlockOperandPtrPtr.get!_OperationPtr_setParentWithCheck {operandPtr : BlockOperandPtrPtr} :
+    op'.setParentWithCheck ctx newParent selfIn = some newCtx →
+    operandPtr.get! newCtx = operandPtr.get! ctx := by
+  grind
+
+grind_pattern BlockOperandPtrPtr.get!_OperationPtr_setParentWithCheck =>
+  op'.setParentWithCheck ctx newParent selfIn, some newCtx, operandPtr.get! newCtx
+
+@[simp]
+theorem BlockPtr.getNumArguments!_OperationPtr_setParentWithCheck {block : BlockPtr} :
+    op'.setParentWithCheck ctx newParent selfIn = some newCtx →
+    block.getNumArguments! newCtx = block.getNumArguments! ctx := by
+  grind
+
+grind_pattern BlockPtr.getNumArguments!_OperationPtr_setParentWithCheck =>
+  op'.setParentWithCheck ctx newParent selfIn, some newCtx, block.getNumArguments! newCtx
+
+@[simp]
+theorem BlockArgumentPtr.get!_OperationPtr_setParentWithCheck {blockArg : BlockArgumentPtr} :
+    op'.setParentWithCheck ctx newParent selfIn = some newCtx →
+    blockArg.get! newCtx = blockArg.get! ctx := by
+  grind
+
+grind_pattern BlockArgumentPtr.get!_OperationPtr_setParentWithCheck =>
+  op'.setParentWithCheck ctx newParent selfIn, some newCtx, blockArg.get! newCtx
+
+@[simp]
+theorem RegionPtr.get!_OperationPtr_setParentWithCheck {region : RegionPtr} :
+    op'.setParentWithCheck ctx newParent selfIn = some newCtx →
+    region.get! newCtx = region.get! ctx := by
+  grind
+
+grind_pattern RegionPtr.get!_OperationPtr_setParentWithCheck =>
+  op'.setParentWithCheck ctx newParent selfIn, some newCtx, region.get! newCtx
+
+@[simp]
+theorem ValuePtr.getFirstUse!_OperationPtr_setParentWithCheck {value : ValuePtr} :
+    op'.setParentWithCheck ctx newParent selfIn = some newCtx →
+    value.getFirstUse! newCtx = value.getFirstUse! ctx := by
+  grind
+
+grind_pattern ValuePtr.getFirstUse!_OperationPtr_setParentWithCheck =>
+  op'.setParentWithCheck ctx newParent selfIn, some newCtx, value.getFirstUse! newCtx
+
+@[simp] -- No grind because of Unit
+theorem ValuePtr.getType!_OperationPtr_setParentWithCheck {value : ValuePtr} :
+    op'.setParentWithCheck ctx newParent selfIn = some newCtx →
+    value.getType! newCtx = value.getType! ctx := by
+  grind
+
+grind_pattern ValuePtr.getType!_OperationPtr_setParentWithCheck =>
+  op'.setParentWithCheck ctx newParent selfIn, some newCtx, value.getType! newCtx
+
+@[simp]
+theorem OpOperandPtrPtr.get!_OperationPtr_setParentWithCheck {opOperandPtr : OpOperandPtrPtr} :
+    op'.setParentWithCheck ctx newParent selfIn = some newCtx →
+    opOperandPtr.get! newCtx = opOperandPtr.get! ctx := by
+  grind
+
+grind_pattern OpOperandPtrPtr.get!_OperationPtr_setParentWithCheck =>
+  op'.setParentWithCheck ctx newParent selfIn, some newCtx, opOperandPtr.get! newCtx
+
+end setParentWithCheck
+
+section linkBetweenWithParent
+
+/- OperationPtr.linkBetweenWithParent -/
+attribute [local grind] OperationPtr.linkBetweenWithParent
+
+@[simp]
+theorem IRContext.topLevelOp_OperationPtr_linkBetweenWithParent :
+    op'.linkBetweenWithParent ctx prev next parent selfIn prevIn nextIn parentIn = some newCtx →
+    newCtx.topLevelOp = ctx.topLevelOp := by
+  grind
+
+grind_pattern IRContext.topLevelOp_OperationPtr_linkBetweenWithParent =>
+  op'.linkBetweenWithParent ctx prev next parent selfIn prevIn nextIn parentIn, some newCtx, newCtx.topLevelOp
+
+ --   * Block.firstUse
+ --   * Block.prev
+ --   * Block.next
+ --   * Block.parent
+ --   * Block.firstOp
+ --   * Block.lastOp
+
+@[simp]
+theorem BlockPtr.firstUse!_OperationPtr_linkBetweenWithParent {block : BlockPtr} :
+    op'.linkBetweenWithParent ctx prev next parent selfIn prevIn nextIn parentIn = some newCtx →
+    (block.get! newCtx).firstUse = (block.get! ctx).firstUse
     := by
-  unfold OperationPtr.setParentWithCheck at heq
   grind
 
-@[simp, grind =]
-theorem OperationPtr.getNumResults_OpOperandPtr_setBack :
-    OperationPtr.getNumResults op (OpOperandPtr.setBack operandPtr ctx h₁ v) hop =
-    OperationPtr.getNumResults op ctx (by grind) := by
+grind_pattern BlockPtr.firstUse!_OperationPtr_linkBetweenWithParent =>
+  op'.linkBetweenWithParent ctx prev next parent selfIn prevIn nextIn parentIn, some newCtx, (block.get! newCtx).firstUse
+
+@[simp]
+theorem BlockPtr.prev!_OperationPtr_linkBetweenWithParent {block : BlockPtr} :
+    op'.linkBetweenWithParent ctx prev next parent selfIn prevIn nextIn parentIn = some newCtx →
+    (block.get! newCtx).prev = (block.get! ctx).prev
+    := by
   grind
 
-@[simp, grind =>]
-theorem OpOperandPtr.get!_OperationPtr_setParentWithCheck (res : OpOperandPtr)
-    (heq : operation.setParentWithCheck ctx h' newNext = some newCtx) :
-    res.get! newCtx = res.get! ctx := by
-  grind [OperationPtr.setParentWithCheck]
+grind_pattern BlockPtr.prev!_OperationPtr_linkBetweenWithParent =>
+  op'.linkBetweenWithParent ctx prev next parent selfIn prevIn nextIn parentIn, some newCtx, (block.get! newCtx).prev
 
-
-@[simp, grind =]
-theorem ValuePtr.get_OpOperandPtr_pushResult(arg : BlockArgumentPtr)
-    (h : arg.InBounds (operation.pushResult ctx newResult hop)) :
-    arg.get (operation.pushResult ctx newResult hop) h = arg.get ctx := by
+@[simp]
+theorem BlockPtr.next!_OperationPtr_linkBetweenWithParent {block : BlockPtr} :
+    op'.linkBetweenWithParent ctx prev next parent selfIn prevIn nextIn parentIn = some newCtx →
+    (block.get! newCtx).next = (block.get! ctx).next
+    := by
   grind
 
+grind_pattern BlockPtr.next!_OperationPtr_linkBetweenWithParent =>
+  op'.linkBetweenWithParent ctx prev next parent selfIn prevIn nextIn parentIn, some newCtx, (block.get! newCtx).next
 
-@[simp, grind =>]
-theorem BlockArgumentPtr.get!_OperationPtr_setParentWithCheck (res : BlockArgumentPtr)
-    (heq : operation.setParentWithCheck ctx h' newNext = some newCtx) :
-    res.get! newCtx = res.get! ctx  := by
-  grind [OperationPtr.setParentWithCheck]
-
-
-@[simp, grind =>]
-theorem RegionPtr.get!_OperationPtr_setParentWithCheck (rg : RegionPtr)
-    (heq : operation.setParentWithCheck ctx h' newNext = some newCtx) :
-    rg.get! newCtx = rg.get! ctx  := by
-  grind [OperationPtr.setParentWithCheck]
-
-@[simp, grind =>]
-theorem BlockArgumentPtr.get_OperationPtr_setParentWithCheck (res : BlockArgumentPtr) (h : res.InBounds ctx)
-    (heq : operation.setParentWithCheck ctx h' newNext = some newCtx) :
-    res.get newCtx (by grind) = res.get ctx := by
-  grind [OperationPtr.setParentWithCheck]
-
-
-@[simp, grind =>]
-theorem OpResultPtr.get!_OperationPtr_setParentWithCheck (res : OpResultPtr)
-    (heq : operation.setParentWithCheck ctx h' newNext = some newCtx) :
-    res.get! newCtx = res.get! ctx := by
-  grind [OperationPtr.setParentWithCheck]
-
-
-variable (ctx : IRContext)
-variable (ctxInBounds : ctx.FieldsInBounds)
-
-@[simp, grind .]
-theorem OperationPtr.get!_OpOperandPtr_setBack_results_size (op : OperationPtr):
-    op.getNumResults! (OpOperandPtr.setBack operandPtr ctx h newBack) = op.getNumResults! ctx := by
-  grind [OpOperandPtr.setBack]
-
-@[simp, grind .]
-theorem OperationPtr.get!_OpOperandPtr_setNextUse_results_size (op : OperationPtr):
-    op.getNumResults! (OpOperandPtr.setNextUse operandPtr ctx h newNextUse) = op.getNumResults! ctx := by
-  grind [OpOperandPtr.setNextUse]
-
-@[simp, grind .]
-theorem OperationPtr.get!_ValuePtr_setFirstUse_results_size (op : OperationPtr) :
-    op.getNumResults! (ValuePtr.setFirstUse val ctx h newFirstUse) = op.getNumResults! ctx := by
-  cases val <;> grind [ValuePtr.setFirstUse]
-
-@[simp, grind =]
-theorem OpOperandPtr.OperationPtr_get!_setBack_operands_size (op : OperationPtr) :
-    op.getNumOperands! (OpOperandPtr.setBack operandPtr ctx h₁ v) =
-    op.getNumOperands! ctx := by
-  grind [OpOperandPtr.get, OperationPtr.get!]
-
-@[simp, grind =]
-theorem OpOperandPtr.OperationPtr_get!_setNextUse_operands_size (op : OperationPtr) :
-    op.getNumOperands! (OpOperandPtr.setNextUse operandPtr ctx h₁ v) =
-    op.getNumOperands! ctx := by
-  grind [OpOperandPtr.get, OperationPtr.get!]
-
-@[simp, grind =]
-theorem OpOperandPtr.OperationPtr_get!_setFirstUse_operands_size (op : OperationPtr) :
-    op.getNumOperands! (ValuePtr.setFirstUse valuePtr ctx h₁ v) =
-    op.getNumOperands! ctx := by
-  cases valuePtr <;> grind [OpOperandPtr.get, OperationPtr.get!]
-
-@[simp, grind =]
-theorem OpOperandPtr.OperationPtr_get!_setBack_operands_owner (opr : OpOperandPtr) :
-    (opr.get! (OpOperandPtr.setBack operandPtr ctx h₁ v)).owner =
-    (opr.get! ctx).owner := by
-  grind [OpOperandPtr.get, OperationPtr.get!]
-
-@[simp, grind =]
-theorem OpOperandPtr.OperationPtr_get!_setNextUse_operands_owner (opr : OpOperandPtr) :
-    (opr.get! (OpOperandPtr.setNextUse operandPtr ctx h₁ v)).owner =
-    (opr.get! ctx).owner := by
-  grind [OpOperandPtr.get, OperationPtr.get!]
-
-@[simp, grind =]
-theorem OpOperandPtr.OperationPtr_get!_setFirstUse_operands_owner (opr : OpOperandPtr) :
-    (opr.get! (ValuePtr.setFirstUse valuePtr ctx h₁ v)).owner =
-    (opr.get! ctx).owner := by
-  cases valuePtr <;> grind [OpOperandPtr.get, OperationPtr.get!]
-
-@[simp, grind =]
-theorem OpResultPtr.get!_OpOperandPtr_linkBetween (res : OpResultPtr) (op : OperationPtr) (h₁ : op.InBounds ctx) :
-    res.get! (op.linkBetween ctx prevOp nextOp h₁ h₂ h₃) = res.get! ctx := by
-  unfold OperationPtr.linkBetween
-  simp
-  split
-  · split <;> grind
-  · grind
-
-@[simp, grind =]
-theorem BlockArgumentPtr.get!_OpOperandPtr_linkBetween (res : BlockArgumentPtr) (op : OperationPtr) (h₁ : op.InBounds ctx) :
-    res.get! (op.linkBetween ctx prevOp nextOp h₁ h₂ h₃) = res.get! ctx := by
-  unfold OperationPtr.linkBetween
-  simp
-  split
-  · split <;> grind
-  · grind
-
-@[simp, grind =]
-theorem ValuePtr.get!_OpOperandPtr_linkBetween (res : ValuePtr) (op : OperationPtr) (h₁ : op.InBounds ctx) :
-    res.getFirstUse! (op.linkBetween ctx prevOp nextOp h₁ h₂ h₃) = res.getFirstUse! ctx := by
-  cases res <;> grind [getFirstUse!]
-
-@[simp, grind =]
-theorem OpOperandPtr.get!_OpOperandPtr_linkBetween (res : OpOperandPtr) (op : OperationPtr) (h₁ : op.InBounds ctx) :
-    res.get! (op.linkBetween ctx prevOp nextOp h₁ h₂ h₃) = res.get! ctx := by
-  unfold OperationPtr.linkBetween
-  simp
-  split
-  · split <;> grind
-  · grind
-
-@[simp, grind =>]
-theorem OpResultPtr.get!_OpOperandPtr_linkBetweenWithParent (res : OpResultPtr) (op : OperationPtr) (h₁ : op.InBounds ctx)
-    (heq : op.linkBetweenWithParent ctx prevOp nextOp parent hp h₁ h₂ h₃ = some newCtx) :
-    res.get! newCtx = res.get! ctx := by
-  unfold OperationPtr.linkBetweenWithParent at heq
+@[simp]
+theorem BlockPtr.parent!_OperationPtr_linkBetweenWithParent {block : BlockPtr} :
+    op'.linkBetweenWithParent ctx prev next parent selfIn prevIn nextIn parentIn = some newCtx →
+    (block.get! newCtx).parent = (block.get! ctx).parent := by
   grind
 
-@[simp, grind =>]
-theorem BlockArgumentPtr.get!_OpOperandPtr_linkBetweenWithParent (res : BlockArgumentPtr)  (op : OperationPtr) (h₁ : op.InBounds ctx)
-    (heq : op.linkBetweenWithParent ctx prevOp nextOp parent hp h₁ h₂ h₃ = some newCtx) :
-    res.get! newCtx = res.get! ctx := by
-  unfold OperationPtr.linkBetweenWithParent at heq
+grind_pattern BlockPtr.parent!_OperationPtr_linkBetweenWithParent =>
+  op'.linkBetweenWithParent ctx prev next parent selfIn prevIn nextIn parentIn, some newCtx, (block.get! newCtx).parent
+
+theorem BlockPtr.firstOp!_OperationPtr_linkBetweenWithParent {block : BlockPtr} :
+    op'.linkBetweenWithParent ctx prev next parent selfIn prevIn nextIn parentIn = some newCtx →
+    (block.get! newCtx).firstOp =
+    if parent = block ∧ prev = none then
+      some op'
+    else
+      (block.get! ctx).firstOp := by
   grind
 
-@[simp, grind =>]
-theorem ValuePtr.get!_OpOperandPtr_linkBetweenWithParent (res : ValuePtr)  (op : OperationPtr) (h₁ : op.InBounds ctx)
-    (heq : op.linkBetweenWithParent ctx prevOp nextOp parent hp h₁ h₂ h₃ = some newCtx) :
-    res.getFirstUse! newCtx = res.getFirstUse! ctx := by
-  cases res <;> grind [getFirstUse!]
+grind_pattern BlockPtr.firstOp!_OperationPtr_linkBetweenWithParent =>
+  op'.linkBetweenWithParent ctx prev next parent selfIn prevIn nextIn parentIn, some newCtx, (block.get! newCtx).firstOp
 
-@[simp, grind =>]
-theorem OpOperandPtr.get!_OpOperandPtr_linkBetweenWithParent (res : OpOperandPtr) (op : OperationPtr) (h₁ : op.InBounds ctx)
-    (heq : op.linkBetweenWithParent ctx prevOp nextOp parent hp h₁ h₂ h₃ = some newCtx) :
-    res.get! newCtx = res.get! ctx := by
-  unfold OperationPtr.linkBetweenWithParent at heq
+theorem BlockPtr.lastOp!_OperationPtr_linkBetweenWithParent {block : BlockPtr} :
+    op'.linkBetweenWithParent ctx prev next parent selfIn prevIn nextIn parentIn = some newCtx →
+    (block.get! newCtx).lastOp =
+    if parent = block ∧ next = none then
+      some op'
+    else
+      (block.get! ctx).lastOp := by
   grind
 
-@[simp, grind =]
-theorem OpResultPtr.get_OpOperandPtr_linkBetween (res : OpResultPtr) (h : res.InBounds ctx) (op : OperationPtr) (h₁ : op.InBounds ctx) :
-    res.get (op.linkBetween ctx prevOp nextOp h₁ h₂ h₃) (by grind) = res.get ctx h := by
-  have := @get!_OpOperandPtr_linkBetween ctx prevOp nextOp h₂ h₃ res
+grind_pattern BlockPtr.lastOp!_OperationPtr_linkBetweenWithParent =>
+  op'.linkBetweenWithParent ctx prev next parent selfIn prevIn nextIn parentIn, some newCtx, (block.get! newCtx).lastOp
+
+theorem OperationPtr.prev!_OperationPtr_linkBetweenWithParent {operation : OperationPtr} :
+    op'.linkBetweenWithParent ctx prev next parent selfIn prevIn nextIn parentIn = some newCtx →
+    (operation.get! newCtx).prev =
+    if operation = next then
+      some op'
+    else if operation = op' then
+      prev
+    else
+      (operation.get! ctx).prev := by
   grind
 
-@[simp, grind =]
-theorem BlockArgumentPtr.get_OpOperandPtr_linkBetween (res : BlockArgumentPtr) (h : res.InBounds ctx) (op : OperationPtr) (h₁ : op.InBounds ctx) :
-    res.get (op.linkBetween ctx prevOp nextOp h₁ h₂ h₃) (by grind) = res.get ctx h := by
-  have := @get!_OpOperandPtr_linkBetween ctx prevOp nextOp h₂ h₃ res
+grind_pattern OperationPtr.prev!_OperationPtr_linkBetweenWithParent =>
+  op'.linkBetweenWithParent ctx prev next parent selfIn prevIn nextIn parentIn, some newCtx, (operation.get! newCtx).prev
+
+theorem OperationPtr.next!_OperationPtr_linkBetweenWithParent {operation : OperationPtr} :
+    op'.linkBetweenWithParent ctx prev next parent selfIn prevIn nextIn parentIn = some newCtx →
+    (operation.get! newCtx).next =
+    if operation = prev then
+      some op'
+    else if operation = op' then
+      next
+    else
+      (operation.get! ctx).next := by
   grind
 
-@[simp, grind =]
-theorem ValuePtr.get_OpOperandPtr_linkBetween (res : ValuePtr) (h : res.InBounds ctx) (op : OperationPtr) (h₁ : op.InBounds ctx) :
-    res.getFirstUse (op.linkBetween ctx prevOp nextOp h₁ h₂ h₃) (by grind) = res.getFirstUse ctx h := by
-  have := @get!_OpOperandPtr_linkBetween ctx prevOp nextOp h₂ h₃ res
+grind_pattern OperationPtr.next!_OperationPtr_linkBetweenWithParent =>
+  op'.linkBetweenWithParent ctx prev next parent selfIn prevIn nextIn parentIn, some newCtx, (operation.get! newCtx).next
+
+theorem OperationPtr.parent!_OperationPtr_linkBetweenWithParent {operation : OperationPtr} :
+    op'.linkBetweenWithParent ctx prev next parent selfIn prevIn nextIn parentIn = some newCtx →
+    (operation.get! newCtx).parent =
+    if operation = op' then
+      some parent
+    else
+      (operation.get! ctx).parent := by
   grind
 
-@[simp, grind =]
-theorem OpOperandPtr.get_OpOperandPtr_linkBetween (res : OpOperandPtr) (h : res.InBounds ctx) (op : OperationPtr) (h₁ : op.InBounds ctx) :
-    res.get (op.linkBetween ctx prevOp nextOp h₁ h₂ h₃) (by grind) = res.get ctx h := by
-  have := @get!_OpOperandPtr_linkBetween ctx prevOp nextOp h₂ h₃ res
+grind_pattern OperationPtr.parent!_OperationPtr_linkBetweenWithParent =>
+  op'.linkBetweenWithParent ctx prev next parent selfIn prevIn nextIn parentIn, some newCtx, (operation.get! newCtx).parent
+
+@[simp]
+theorem OperationPtr.opType!_OperationPtr_linkBetweenWithParent {operation : OperationPtr} :
+    op'.linkBetweenWithParent ctx prev next parent selfIn prevIn nextIn parentIn = some newCtx →
+    (operation.get! newCtx).opType = (operation.get! ctx).opType := by
   grind
 
-@[simp, grind =]
-theorem OperationPtr.getParent_OperationPtr_linkBetween :
-    (OperationPtr.get op (OperationPtr.linkBetween op' ctx prevOp nextOp h₁ h₂ h₃) hop).parent =
-      (OperationPtr.get op ctx (by grind)).parent := by
-  unfold OperationPtr.linkBetween
+grind_pattern OperationPtr.opType!_OperationPtr_linkBetweenWithParent =>
+  op'.linkBetweenWithParent ctx prev next parent selfIn prevIn nextIn parentIn, some newCtx, (operation.get! newCtx).opType
+
+@[simp]
+theorem OperationPtr.attrs!_OperationPtr_linkBetweenWithParent {operation : OperationPtr} :
+    op'.linkBetweenWithParent ctx prev next parent selfIn prevIn nextIn parentIn = some newCtx →
+    (operation.get! newCtx).attrs = (operation.get! ctx).attrs := by
   grind
 
-@[simp, grind =>]
-theorem OpResultPtr.get_OpOperandPtr_linkBetweenWithParent (res : OpResultPtr) (h : res.InBounds ctx) (op : OperationPtr) (h₁ : op.InBounds ctx)
-    (heq : op.linkBetweenWithParent ctx prevOp nextOp parent hp h₁ h₂ h₃ = some newCtx) :
-    res.get newCtx (by grind) = res.get ctx h := by
-  have := get!_OpOperandPtr_linkBetweenWithParent (heq := heq)
+grind_pattern OperationPtr.attrs!_OperationPtr_linkBetweenWithParent =>
+  op'.linkBetweenWithParent ctx prev next parent selfIn prevIn nextIn parentIn, some newCtx, (operation.get! newCtx).attrs
+
+@[simp]
+theorem OperationPtr.properties!_OperationPtr_linkBetweenWithParent {operation : OperationPtr} :
+    op'.linkBetweenWithParent ctx prev next parent selfIn prevIn nextIn parentIn = some newCtx →
+    (operation.get! newCtx).properties = (operation.get! ctx).properties := by
   grind
 
+grind_pattern OperationPtr.properties!_OperationPtr_linkBetweenWithParent =>
+  op'.linkBetweenWithParent ctx prev next parent selfIn prevIn nextIn parentIn, some newCtx, (operation.get! newCtx).properties
 
-@[simp, grind =>]
-theorem BlockArgumentPtr.get_OpOperandPtr_linkBetweenWithParent (res : BlockArgumentPtr) (h : res.InBounds ctx) (op : OperationPtr) (h₁ : op.InBounds ctx)
-    (heq : op.linkBetweenWithParent ctx prevOp nextOp parent hp h₁ h₂ h₃ = some newCtx) :
-    res.get newCtx (by grind) = res.get ctx h := by
-  have := get!_OpOperandPtr_linkBetweenWithParent (heq := heq) (res := res)
+@[simp]
+theorem OperationPtr.getNumResults!_OperationPtr_linkBetweenWithParent {operation : OperationPtr} :
+    op'.linkBetweenWithParent ctx prev next parent selfIn prevIn nextIn parentIn = some newCtx →
+    operation.getNumResults! newCtx = operation.getNumResults! ctx := by
   grind
 
-@[simp, grind =>]
-theorem ValuePtr.get_OpOperandPtr_linkBetweenWithParent (res : ValuePtr) (h : res.InBounds ctx) (op : OperationPtr) (h₁ : op.InBounds ctx)
-    (heq : op.linkBetweenWithParent ctx prevOp nextOp parent hp h₁ h₂ h₃ = some newCtx) :
-    res.getFirstUse newCtx (by grind) = res.getFirstUse ctx h := by
-  have := get!_OpOperandPtr_linkBetweenWithParent (heq := heq) (res := res)
+grind_pattern OperationPtr.getNumResults!_OperationPtr_linkBetweenWithParent =>
+  op'.linkBetweenWithParent ctx prev next parent selfIn prevIn nextIn parentIn, some newCtx, operation.getNumResults! newCtx
+
+@[simp]
+theorem OpResultPtr.get!_OperationPtr_linkBetweenWithParent {opResult : OpResultPtr} :
+    op'.linkBetweenWithParent ctx prev next parent selfIn prevIn nextIn parentIn = some newCtx →
+    opResult.get! newCtx = opResult.get! ctx := by
   grind
 
-@[simp, grind =>]
-theorem OpOperandPtr.get_OpOperandPtr_linkBetweenWithParent (res : OpOperandPtr) (h : res.InBounds ctx) (op : OperationPtr) (h₁ : op.InBounds ctx)
-    (heq : op.linkBetweenWithParent ctx prevOp nextOp parent hp h₁ h₂ h₃ = some newCtx) :
-    res.get newCtx (by grind) = res.get ctx h := by
-  have := get!_OpOperandPtr_linkBetweenWithParent (heq := heq) (res := res)
+grind_pattern OpResultPtr.get!_OperationPtr_linkBetweenWithParent =>
+  op'.linkBetweenWithParent ctx prev next parent selfIn prevIn nextIn parentIn, some newCtx, opResult.get! newCtx
+
+@[simp]
+theorem OperationPtr.getNumOperands!_OperationPtr_linkBetweenWithParent {operation : OperationPtr} :
+    op'.linkBetweenWithParent ctx prev next parent selfIn prevIn nextIn parentIn = some newCtx →
+    operation.getNumOperands! newCtx = operation.getNumOperands! ctx := by
   grind
+
+grind_pattern OperationPtr.getNumOperands!_OperationPtr_linkBetweenWithParent =>
+  op'.linkBetweenWithParent ctx prev next parent selfIn prevIn nextIn parentIn, some newCtx, operation.getNumOperands! newCtx
+
+@[simp]
+theorem OpOperandPtr.get!_OperationPtr_linkBetweenWithParent {operand : OpOperandPtr} :
+    op'.linkBetweenWithParent ctx prev next parent selfIn prevIn nextIn parentIn = some newCtx →
+    operand.get! newCtx = operand.get! ctx := by
+  grind
+
+grind_pattern OpOperandPtr.get!_OperationPtr_linkBetweenWithParent =>
+  op'.linkBetweenWithParent ctx prev next parent selfIn prevIn nextIn parentIn, some newCtx, operand.get! newCtx
+
+@[simp]
+theorem OperationPtr.getNumSuccessors!_OperationPtr_linkBetweenWithParent {operation : OperationPtr} :
+    op'.linkBetweenWithParent ctx prev next parent selfIn prevIn nextIn parentIn = some newCtx →
+    operation.getNumSuccessors! newCtx = operation.getNumSuccessors! ctx := by
+  grind
+
+grind_pattern OperationPtr.getNumSuccessors!_OperationPtr_linkBetweenWithParent =>
+  op'.linkBetweenWithParent ctx prev next parent selfIn prevIn nextIn parentIn, some newCtx, operation.getNumSuccessors! newCtx
+
+@[simp]
+theorem BlockOperandPtr.get!_OperationPtr_linkBetweenWithParent {operand : BlockOperandPtr} :
+    op'.linkBetweenWithParent ctx prev next parent selfIn prevIn nextIn parentIn = some newCtx →
+    operand.get! newCtx = operand.get! ctx := by
+  grind
+
+grind_pattern BlockOperandPtr.get!_OperationPtr_linkBetweenWithParent =>
+  op'.linkBetweenWithParent ctx prev next parent selfIn prevIn nextIn parentIn, some newCtx, operand.get! newCtx
+
+@[simp]
+theorem OperationPtr.getNumRegions!_OperationPtr_linkBetweenWithParent {operation : OperationPtr} :
+    op'.linkBetweenWithParent ctx prev next parent selfIn prevIn nextIn parentIn = some newCtx →
+    operation.getNumRegions! newCtx = operation.getNumRegions! ctx := by
+  grind
+
+grind_pattern OperationPtr.getNumRegions!_OperationPtr_linkBetweenWithParent =>
+  op'.linkBetweenWithParent ctx prev next parent selfIn prevIn nextIn parentIn, some newCtx, operation.getNumRegions! newCtx
+
+@[simp]
+theorem OperationPtr.getRegion!_OperationPtr_linkBetweenWithParent {operation : OperationPtr} :
+    op'.linkBetweenWithParent ctx prev next parent selfIn prevIn nextIn parentIn = some newCtx →
+    operation.getRegion! newCtx = operation.getRegion! ctx := by
+  grind
+
+grind_pattern OperationPtr.getRegion!_OperationPtr_linkBetweenWithParent =>
+  op'.linkBetweenWithParent ctx prev next parent selfIn prevIn nextIn parentIn, some newCtx, operation.getRegion! newCtx
+
+@[simp]
+theorem BlockOperandPtrPtr.get!_OperationPtr_linkBetweenWithParent {operandPtr : BlockOperandPtrPtr} :
+    op'.linkBetweenWithParent ctx prev next parent selfIn prevIn nextIn parentIn = some newCtx →
+    operandPtr.get! newCtx = operandPtr.get! ctx := by
+  grind
+
+grind_pattern BlockOperandPtrPtr.get!_OperationPtr_linkBetweenWithParent =>
+  op'.linkBetweenWithParent ctx prev next parent selfIn prevIn nextIn parentIn, some newCtx, operandPtr.get! newCtx
+
+@[simp]
+theorem BlockPtr.getNumArguments!_OperationPtr_linkBetweenWithParent {block : BlockPtr} :
+    op'.linkBetweenWithParent ctx prev next parent selfIn prevIn nextIn parentIn = some newCtx →
+    block.getNumArguments! newCtx = block.getNumArguments! ctx := by
+  grind
+
+grind_pattern BlockPtr.getNumArguments!_OperationPtr_linkBetweenWithParent =>
+  op'.linkBetweenWithParent ctx prev next parent selfIn prevIn nextIn parentIn, some newCtx, block.getNumArguments! newCtx
+
+@[simp]
+theorem BlockArgumentPtr.get!_OperationPtr_linkBetweenWithParent {blockArg : BlockArgumentPtr} :
+    op'.linkBetweenWithParent ctx prev next parent selfIn prevIn nextIn parentIn = some newCtx →
+    blockArg.get! newCtx = blockArg.get! ctx := by
+  grind
+
+grind_pattern BlockArgumentPtr.get!_OperationPtr_linkBetweenWithParent =>
+  op'.linkBetweenWithParent ctx prev next parent selfIn prevIn nextIn parentIn, some newCtx, blockArg.get! newCtx
+
+@[simp]
+theorem RegionPtr.get!_OperationPtr_linkBetweenWithParent {region : RegionPtr} :
+    op'.linkBetweenWithParent ctx prev next parent selfIn prevIn nextIn parentIn = some newCtx →
+    region.get! newCtx = region.get! ctx := by
+  grind
+
+grind_pattern RegionPtr.get!_OperationPtr_linkBetweenWithParent =>
+  op'.linkBetweenWithParent ctx prev next parent selfIn prevIn nextIn parentIn, some newCtx, region.get! newCtx
+
+@[simp]
+theorem ValuePtr.getFirstUse!_OperationPtr_linkBetweenWithParent {value : ValuePtr} :
+    op'.linkBetweenWithParent ctx prev next parent selfIn prevIn nextIn parentIn = some newCtx →
+    value.getFirstUse! newCtx = value.getFirstUse! ctx := by
+  grind
+
+grind_pattern ValuePtr.getFirstUse!_OperationPtr_linkBetweenWithParent =>
+  op'.linkBetweenWithParent ctx prev next parent selfIn prevIn nextIn parentIn, some newCtx, value.getFirstUse! newCtx
+
+theorem ValuePtr.getType!_OperationPtr_linkBetweenWithParent {value : ValuePtr} :
+    op'.linkBetweenWithParent ctx prev next parent selfIn prevIn nextIn parentIn = some newCtx →
+    value.getType! newCtx = value.getType! ctx := by
+  grind
+
+grind_pattern ValuePtr.getType!_OperationPtr_linkBetweenWithParent =>
+  op'.linkBetweenWithParent ctx prev next parent selfIn prevIn nextIn parentIn, some newCtx, value.getType! newCtx
+
+@[simp]
+theorem OpOperandPtrPtr.get!_OperationPtr_linkBetweenWithParent {opOperandPtr : OpOperandPtrPtr} :
+    op'.linkBetweenWithParent ctx prev next parent selfIn prevIn nextIn parentIn = some newCtx →
+    opOperandPtr.get! newCtx = opOperandPtr.get! ctx := by
+  grind
+
+grind_pattern OpOperandPtrPtr.get!_OperationPtr_linkBetweenWithParent =>
+  op'.linkBetweenWithParent ctx prev next parent selfIn prevIn nextIn parentIn, some newCtx, opOperandPtr.get! newCtx
+
+end linkBetweenWithParent
